Bet/Tests/Redeem.fsx
@@ -1,0 +1,61 @@
+#load "Bet.fsx"
+
+open Bet
+
+module Asset = Consensus.Asset
+module Contract = Consensus.Contract
+module Hash = Consensus.Hash
+module Result = Infrastructure.Result
+module Tx = Consensus.TxSkeleton
+module Types = Consensus.Types
+
+//////////////////////////////////////////////////////////////////////////
+// Redeem with only returnAddress fails
+//////////////////////////////////////////////////////////////////////////
+
+match redeem emptyTx onlyReturnAddress emptyWallet with
+| Error "Could not parse Price from messageBody" ->
+    printfn "OK: Redeem with only returnAddress fails"
+| Ok cr -> failwithf "Should not return ok without Price! Got ContractReturn `%A`" cr
+| Error e -> failwithf "Failed with unexpected error: `%A`" e
+
+//////////////////////////////////////////////////////////////////////////
+// Redeem with only Price fails
+//////////////////////////////////////////////////////////////////////////
+
+match redeem emptyTx onlyPrice emptyWallet with
+| Error "Could not parse returnAddress from messageBody" ->
+    printfn "OK: Redeem with only Price fails"
+| Ok cr -> failwithf "Should not return ok without returnAddress! Got ContractReturn `%A`" cr
+| Error e -> failwithf "Failed with unexpected error: `%A`" e
+
+//////////////////////////////////////////////////////////////////////////
+// Redeem succeeds with OK Data
+//////////////////////////////////////////////////////////////////////////
+
+let okData = mkData returnAddress strike
+let tx1Bull =
+    mkTx [(mkInput contractLock bullToken 1UL)] []
+match redeem tx1Bull okData wallet50ZP with
+| Ok tx ->
+    printfn "OK: Redeem succeeds with OK Data"
+| Error e -> failwithf "Failed with unexpected error: `%A`" e
+
+/////////////////////////////////////////////////////////////////////////////
+// Redeem with bull token fails with low strike, but succeeds with bear token
+/////////////////////////////////////////////////////////////////////////////
+
+let lowStrike = mkData returnAddress (strike-1UL)
+let tx25Bull = mkTx [(mkInput contractLock bullToken 25UL)] []
+let tx25Bear = mkTx [(mkInput contractLock bearToken 25UL)] []
+
+match redeem tx25Bull lowStrike wallet50ZP with
+| Error "Could not construct tx from wallet" ->
+    printfn "OK: Redeem with bull tokens fails for low strike"
+| Ok cr -> failwithf "Should not return ok! Got ContractReturn `%A`" cr
+| Error e -> failwithf "Failed with unexpected error: `%A`" e
+
+match redeem tx25Bear lowStrike wallet50ZP with
+| Ok tx ->
+    printfn "OK: Redeem with bear tokens succeeds for low strike"
+| Error e -> failwithf "Failed with unexpected error: `%A`" e
